merkle: prove `getBit`

new/proof/github_com/sanjit_bhat/pav/merkle_proof/code.v
@@ -21,29 +21,28 @@ Fixpoint own_tree ptr t d : iProp Σ :=
     "%Heq_ptr" ∷ ⌜ ptr = null ⌝
   | Leaf label val =>
     ∃ sl_hash sl_label sl_val,
-    "Hstruct" ∷ ptr ↦{d}
+    "Hnode" ∷ ptr ↦{d}
       (merkle.node.mk leafNodeTy sl_hash null null sl_label sl_val) ∗
     "#Hsl_hash" ∷ sl_hash ↦*□ hash ∗
     "#Hsl_label" ∷ sl_label ↦*□ label ∗
     "#Hsl_val" ∷ sl_val ↦*□ val
   | Inner child0 child1 =>
     ∃ sl_hash ptr_child0 ptr_child1,
-    "Hstruct" ∷ ptr ↦{d}
+    "Hnode" ∷ ptr ↦{d}
       (merkle.node.mk innerNodeTy sl_hash ptr_child0 ptr_child1 slice.nil slice.nil) ∗
     "#Hsl_hash" ∷ sl_hash ↦*□ hash ∗
     "Hown_child0" ∷ own_tree ptr_child0 child0 d ∗
-    "Hown_child1" ∷ own_tree ptr_child1 child1 d ∗
-    "%Heq_children" ∷ ⌜ ptr_child0 ≠ null ∨ ptr_child1 ≠ null ⌝
+    "Hown_child1" ∷ own_tree ptr_child1 child1 d
   | Cut _ =>
     ∃ sl_hash,
-    "Hstruct" ∷ ptr ↦{d}
+    "Hnode" ∷ ptr ↦{d}
       (merkle.node.mk cutNodeTy sl_hash null null slice.nil slice.nil) ∗
     "#Hsl_hash" ∷ sl_hash ↦*□ hash
   end.
 
 Definition own ptr m d : iProp Σ :=
   ∃ ptr_root t,
-  "Hstruct" ∷ ptr ↦{d} (merkle.Map.mk ptr_root) ∗
+  "HMap" ∷ ptr ↦{d} (merkle.Map.mk ptr_root) ∗
   "%Heq_tree" ∷ ⌜ m = to_map t ⌝ ∗
   "Hown_tree" ∷ own_tree ptr_root t d ∗
   "%His_cutless" ∷ ⌜ is_cutless t ⌝ ∗
@@ -70,11 +69,262 @@ Lemma own_empty_tree t d :
 Proof.
   iIntros "H". destruct t; [done|..];
     iNamed "H"; iNamed "H";
-    (iDestruct (typed_pointsto_not_null with "Hstruct") as %?; [|done]);
+    (iDestruct (typed_pointsto_not_null with "Hnode") as %?; [|done]);
     by rewrite go_type_size_unseal.
 Qed.
 
 (** program proofs. *)
+
+Lemma wp_compLeafHash sl_label sl_val (label val : list w8) :
+  {{{
+    is_pkg_init merkle ∗
+    "#Hsl_label" ∷ sl_label ↦*□ label ∗
+    "#Hsl_val" ∷ sl_val ↦*□ val
+  }}}
+  @! merkle.compLeafHash #sl_label #sl_val
+  {{{
+    sl_hash hash, RET #sl_hash;
+    "Hsl_hash" ∷ sl_hash ↦* hash ∗
+    "#His_hash" ∷ cryptoffi.is_hash
+      (Some $ leafNodeTag ::
+      (u64_le $ length label) ++ label ++
+      (u64_le $ length val) ++ val)
+      hash
+  }}}.
+Proof.
+  wp_start as "@". wp_auto.
+  wp_apply cryptoffi.wp_NewHasher as "* @".
+  wp_apply wp_slice_literal as "* Hsl_b".
+  wp_apply (cryptoffi.wp_Hasher_Write with "[$Hown_hr $Hsl_b]") as "@".
+  iClear "Hsl_b".
+  wp_apply wp_WriteInt as "* [Hsl_b _]".
+  { iDestruct own_slice_nil as "$".
+    iDestruct own_slice_cap_nil as "$". }
+  wp_apply (cryptoffi.wp_Hasher_Write with "[$Hown_hr $Hsl_b]") as "@".
+  iClear "Hsl_b".
+  wp_apply (cryptoffi.wp_Hasher_Write with "[$Hown_hr $Hsl_label]") as "@".
+  iClear "Hsl_b".
+  wp_apply wp_WriteInt as "* [Hsl_b _]".
+  { iDestruct own_slice_nil as "$".
+    iDestruct own_slice_cap_nil as "$". }
+  wp_apply (cryptoffi.wp_Hasher_Write with "[$Hown_hr $Hsl_b]") as "@".
+  iClear "Hsl_b".
+  wp_apply (cryptoffi.wp_Hasher_Write with "[$Hown_hr $Hsl_val]") as "@".
+  iClear "Hsl_b".
+  wp_apply (cryptoffi.wp_Hasher_Sum with "[$Hown_hr]") as "* @".
+  { iDestruct own_slice_nil as "$". }
+
+  list_simplifier.
+  iDestruct (own_slice_len with "Hsl_label") as %->.
+  iDestruct (own_slice_len with "Hsl_val") as %->.
+  iApply "HΦ". iFrame.
+  iExactEq "His_hash".
+  rewrite /named. repeat f_equal; word.
+Qed.
+
+Lemma wp_compInnerHash sl_child0 sl_child1 (child0 child1 : list w8) :
+  {{{
+    is_pkg_init merkle ∗
+    "#Hsl_child0" ∷ sl_child0 ↦*□ child0 ∗
+    "#Hsl_child1" ∷ sl_child1 ↦*□ child1
+  }}}
+  @! merkle.compInnerHash #sl_child0 #sl_child1
+  {{{
+    sl_hash hash, RET #sl_hash;
+    "Hsl_hash" ∷ sl_hash ↦* hash ∗
+    "#His_hash" ∷ cryptoffi.is_hash
+      (Some $ innerNodeTag :: child0 ++ child1)
+      hash
+  }}}.
+Proof.
+  wp_start as "@". wp_auto.
+  wp_apply cryptoffi.wp_NewHasher as "* @".
+  wp_apply wp_slice_literal as "* Hsl_b".
+  wp_apply (cryptoffi.wp_Hasher_Write with "[$Hown_hr $Hsl_b]") as "@".
+  iClear "Hsl_b".
+  wp_apply (cryptoffi.wp_Hasher_Write with "[$Hown_hr $Hsl_child0]") as "@".
+  iClear "Hsl_b".
+  wp_apply (cryptoffi.wp_Hasher_Write with "[$Hown_hr $Hsl_child1]") as "@".
+  iClear "Hsl_b".
+  wp_apply (cryptoffi.wp_Hasher_Sum with "[$Hown_hr]") as "* @".
+  { iDestruct own_slice_nil as "$". }
+  list_simplifier.
+  iApply "HΦ". iFrame "∗#".
+Qed.
+
+Lemma length_bytes_to_bits b :
+  length (bytes_to_bits b) = (8 * length b) % nat.
+Proof.
+  induction b; [done|].
+  rewrite /= IHb. lia.
+Qed.
+(* TODO: add #[global] when upstream. *)
+Hint Rewrite length_bytes_to_bits : len.
+
+Lemma bytes_to_bits_app a b :
+  bytes_to_bits (a ++ b) = bytes_to_bits a ++ bytes_to_bits b.
+Proof. rewrite /bytes_to_bits !fmap_app join_app //. Qed.
+
+Lemma join_lookup_Some_same_length''' {A : Type} ls c i (x : A) :
+  (0 < c)%nat →
+  Forall (λ l, length l = c) ls →
+  mjoin ls !! i = Some x ↔
+  ∃ l, ls !! (i `div` c)%nat = Some l ∧ l !! (i `mod` c)%nat = Some x.
+Proof.
+  intros ??.
+  rewrite {1}(Nat.div_mod_eq i c) (comm Nat.mul).
+  apply join_lookup_Some_same_length'; [done|].
+  apply Nat.mod_upper_bound. lia.
+Qed.
+
+Lemma testbit_spec a n :
+  0 ≤ n →
+  Z.testbit a n = bool_decide (Z.land a (2 ^ n) ≠ 0).
+Proof.
+  intros. case_bool_decide as Heq.
+  - apply Automation.word.decision_assume_opposite.
+    intros Ht. apply Heq. clear Heq. rename Ht into Heq.
+    apply not_true_is_false in Heq.
+    apply Z.bits_inj_iff. intros p.
+    rewrite Z.land_spec Z.bits_0.
+    destruct (decide (p = n)).
+    { subst.
+      rewrite Z.pow2_bits_true; [|word].
+      by rewrite andb_true_r. }
+    rewrite Z.pow2_bits_false; [|word].
+    by rewrite andb_false_r.
+  - apply (f_equal (λ x, Z.testbit x n)) in Heq.
+    rewrite Z.land_spec Z.bits_0 Z.pow2_bits_true in Heq; [|done].
+    by rewrite andb_true_r in Heq.
+Qed.
+
+Lemma lookup_byte_to_bits byt i :
+  (i < 8)%nat →
+  byte_to_bits byt !! i =
+    Some $ bool_decide (word.and byt (word.slu (W8 1) (W8 i)) ≠ W8 0).
+Proof.
+  intros. rewrite /byte_to_bits.
+  assert (∀ x, bool_decide (x ≠ W8 0) = bool_decide (uint.Z x ≠ 0)) as ->.
+  { intros. repeat case_bool_decide; word. }
+  rewrite word.unsigned_and_nowrap.
+  rewrite Automation.word.unsigned_slu'; [|word].
+  rewrite left_id.
+  replace (uint.Z (W8 i)) with (Z.of_nat i) by word.
+  rewrite wrap_small.
+  2: { split; [lia|]. apply Z.pow_lt_mono_r; word. }
+
+  rewrite list_lookup_fmap.
+  rewrite lookup_seqZ_lt; [|lia].
+  rewrite left_id /=.
+  f_equal.
+  rewrite testbit_spec; [done|lia].
+Qed.
+
+Lemma bool_decide_ite_not (P : Prop) {dec : Decision P} :
+  (if bool_decide P then false else true) = bool_decide (¬P).
+Proof. by rewrite bool_decide_not. Qed.
+
+Lemma wp_getBit sl_bs bs (n : w64) :
+  {{{
+    is_pkg_init merkle ∗
+    "#Hsl_bs" ∷ sl_bs ↦*□ bs
+  }}}
+  @! merkle.getBit #sl_bs #n
+  {{{
+    bit, RET #bit;
+    "->" ∷ ⌜ get_bit bs (uint.nat n) = bit ⌝
+  }}}.
+Proof.
+  wp_start as "@". wp_auto.
+  iDestruct (own_slice_len with "Hsl_bs") as %?.
+
+  (* deal with OOB case. *)
+  rewrite /get_bit list_lookup_total_alt.
+  destruct (_ !! _) eqn:Hbs.
+  2:{ apply lookup_ge_None in Hbs.
+    rewrite length_bytes_to_bits in Hbs.
+    wp_if_destruct; [word|].
+    by iApply "HΦ". }
+
+  (* in pure, extract bit. *)
+  opose proof (lookup_lt_Some _ _ _ Hbs) as Hlt_n.
+  rewrite length_bytes_to_bits in Hlt_n.
+  rewrite /bytes_to_bits in Hbs.
+  eapply join_lookup_Some_same_length''' in Hbs as (?&Hb&Ho).
+  3: { apply Forall_fmap, Forall_true. naive_solver. }
+  2: lia.
+  apply list_lookup_fmap_Some in Hb as (byt&->&Hb).
+
+  (* in golang, extract byte. *)
+  wp_if_destruct; [|word].
+  wp_auto.
+  wp_apply (wp_load_slice_elem with "[$Hsl_bs]") as "_".
+  { iPureIntro. exact_eq Hb.
+    f_equal.
+    rewrite word.unsigned_divu_nowrap; [|word].
+    rewrite Z2Nat.inj_div; [done|word..]. }
+
+  (* show equal. *)
+  iApply "HΦ". iPureIntro.
+  rewrite lookup_byte_to_bits in Ho.
+  2: { by apply Nat.mod_upper_bound. }
+  rewrite bool_decide_ite_not.
+  replace (Z.of_nat (uint.nat n `mod` 8)%nat) with (uint.Z n `mod` 8) in Ho.
+  2: { rewrite Nat2Z.inj_mod. word. }
+  simplify_eq/=. clear.
+  assert (∀ x y, x = y → bool_decide (x ≠ W8 0) = bool_decide (y ≠ W8 0))
+    as Ht by naive_solver.
+  f_equal. apply Ht. repeat f_equal. word.
+Qed.
+
+Lemma wp_node_getChild n d nodeTy sl_hash ptr_child0 ptr_child1 sl_label sl_val label (depth : w64) :
+  {{{
+    is_pkg_init merkle ∗
+    "Hnode" ∷ n ↦{d}
+      (merkle.node.mk nodeTy sl_hash ptr_child0 ptr_child1 sl_label sl_val) ∗
+    "#Hsl_label" ∷ sl_label ↦*□ label ∗
+    "%Hlt_depth" ∷ ⌜ uint.Z depth < Z.of_nat (length label) * 8 ⌝
+  }}}
+  n @ (ptrTⁱᵈ merkle.nodeⁱᵈ) @ "getChild" #sl_label #depth
+  {{{
+    ptr_cb ptr_cnb, RET (#ptr_cb, #ptr_cnb);
+    let (cb, cnb) := if get_bit label (uint.nat depth)
+      then (ptr_child1, ptr_child0) else (ptr_child0, ptr_child1) in
+    "Hcb" ∷ ptr_cb ↦{d} cb ∗
+    "Hcnb" ∷ ptr_cnb ↦{d} cnb ∗
+    "Hclose" ∷ (∀ ab anb,
+      ptr_cb ↦{d} ab -∗
+      ptr_cnb ↦{d} anb -∗
+      let (c0, c1) := if get_bit label (uint.nat depth)
+        then (anb, ab) else (ab, anb) in
+      "Hnode" ∷ n ↦{d}
+        (merkle.node.mk nodeTy sl_hash c0 c1 sl_label sl_val))
+  }}}.
+Proof. Admitted.
+
+Lemma wp_put n0 n t depth sl_label sl_val label val :
+  {{{
+    is_pkg_init merkle ∗ is_initialized ∗
+    "Hn0" ∷ n0 ↦ n ∗
+    "Hown_tree" ∷ own_tree n t 1 ∗
+    "#Hlabel" ∷ sl_label ↦*□ label ∗
+    "#Hval" ∷ sl_val ↦*□ val
+  }}}
+  @! merkle.put #n0 #depth #sl_label #sl_val
+  {{{
+    n' t', RET #();
+    let ot' := pure_put t (uint.nat depth) label val in
+    "Hn0" ∷ n0 ↦ n' ∗
+    "%Hsome_tree" ∷ ⌜ ot' = Some t' ⌝ ∗
+    "Hown_tree" ∷ own_tree n' t' 1
+  }}}.
+Proof.
+  wp_start as "[Hinit @]". wp_auto.
+  wp_if_destruct.
+  { iDestruct (own_empty_tree with "Hown_tree") as %->.
+    wp_auto.
+    wp_apply wp_alloc as "* Hnode".
+Admitted.
 
 (*
 Definition wish_Verify (in_tree : bool) label val proof dig : iProp Σ :=
